Squashing Dafny-4 test preview branch here, for final prep and merging with other PRs

Source/DafnyCore/DafnyOptions.cs
@@ -63,8 +63,8 @@ features like traits or co-inductive types.".TrimStart(), "cs");
 
       RegisterLegacyUi(CommonOptionBag.Output, ParseFileInfo, "Compilation options", "out");
       RegisterLegacyUi(CommonOptionBag.UnicodeCharacters, ParseBoolean, "Language feature selection", "unicodeChar", @"
-0 (default) - The char type represents any UTF-16 code unit.
-1 - The char type represents any Unicode scalar value.".TrimStart());
+0 - The char type represents any UTF-16 code unit.
+1 (default) - The char type represents any Unicode scalar value.".TrimStart());
       RegisterLegacyUi(CommonOptionBag.Plugin, ParseStringElement, "Plugins", defaultValue: new List<string>());
       RegisterLegacyUi(CommonOptionBag.Prelude, ParseFileInfo, "Input configuration", "dprelude");
 
@@ -294,8 +294,8 @@ NoGhost - disable printing of functions, ghost methods, and proof
     public bool PrintFunctionCallGraph = false;
     public bool WarnShadowing = false;
     public int DefiniteAssignmentLevel = 1; // [0..2] 2 and 3 have the same effect, 4 turns off an array initialisation check, unless --enforce-determinism is used.
-    public FunctionSyntaxOptions FunctionSyntax = FunctionSyntaxOptions.Version3;
-    public QuantifierSyntaxOptions QuantifierSyntax = QuantifierSyntaxOptions.Version3;
+    public FunctionSyntaxOptions FunctionSyntax = FunctionSyntaxOptions.Version4;
+    public QuantifierSyntaxOptions QuantifierSyntax = QuantifierSyntaxOptions.Version4;
     public HashSet<string> LibraryFiles { get; set; } = new();
     public ContractTestingMode TestContracts = ContractTestingMode.None;
 
@@ -1261,10 +1261,10 @@ Exit code: 0 -- success; 1 -- invalid command-line; 2 -- parse or type errors;
     4. This switch gives early access to the new syntax, and also
     provides a mode to help with migration.
 
-    3 (default) - Compiled functions are written `function method` and
+    3 - Compiled functions are written `function method` and
         `predicate method`. Ghost functions are written `function` and
         `predicate`.
-    4 - Compiled functions are written `function` and `predicate`. Ghost
+    4 (default) - Compiled functions are written `function` and `predicate`. Ghost
         functions are written `ghost function` and `ghost predicate`.
     migration3to4 - Compiled functions are written `function method` and
         `predicate method`. Ghost functions are written `ghost function`
@@ -1294,10 +1294,10 @@ Exit code: 0 -- success; 1 -- invalid command-line; 2 -- parse or type errors;
     <Range>) are allowed. This switch gives early access to the new
     syntax.
 
-    3 (default) - Ranges are only allowed after all quantified variables
+    3 - Ranges are only allowed after all quantified variables
         are declared. (e.g. set x, y | 0 <= x < |s| && y in s[x] && 0 <=
         y :: y)
-    4 - Ranges are allowed after each quantified variable declaration.
+    4 (default) - Ranges are allowed after each quantified variable declaration.
         (e.g. set x | 0 <= x < |s|, y <- s[x] | 0 <= y :: y)
 
     Note that quantifier variable domains (<- <Domain>) are available in
