Source/DafnyCore/Options/CommonOptionBag.cs
@@ -106,7 +106,7 @@ https://github.com/dafny-lang/dafny/blob/master/Source/DafnyLanguageServer/READM
         }
       }
 
-      return QuantifierSyntaxOptions.Version3;
+      return QuantifierSyntaxOptions.Version4;
     }, true, @"
 The syntax for quantification domains is changing from Dafny version 3 to version 4, more specifically where quantifier ranges (|
 <Range>) are allowed. This switch gives early access to the new syntax.
@@ -133,7 +133,7 @@ Note that the C++ backend has various limitations (see Docs/Compilation/Cpp.md).
     ArgumentHelpName = "language",
   };
 
-  public static readonly Option<bool> UnicodeCharacters = new("--unicode-char", () => false,
+  public static readonly Option<bool> UnicodeCharacters = new("--unicode-char", () => true,
     @"
 false - The char type represents any UTF-16 code unit.
 true - The char type represents any Unicode scalar value.".TrimStart()) {
