Test/dafny0/OlderVerification.dfy
@@ -3,43 +3,43 @@
 
 // ----------------------------------
 
-predicate Trivial0(older x: int, s: set<int>) {
+ghost predicate Trivial0(older x: int, s: set<int>) {
   true
 }
 
-predicate Trivial1(older x: int, s: set<int>) {
+ghost predicate Trivial1(older x: int, s: set<int>) {
   x in s
 }
 
-predicate Trivial2(older x: int, s: set<int>) {
+ghost predicate Trivial2(older x: int, s: set<int>) {
   x !in s
 }
 
 // ----------------------------------
 
-predicate Trivial3<X(!new)>(older x: X, s: set<X>) {
+ghost predicate Trivial3<X(!new)>(older x: X, s: set<X>) {
   true
 }
 
-predicate Trivial4<X(!new)>(older x: X, s: set<X>) {
+ghost predicate Trivial4<X(!new)>(older x: X, s: set<X>) {
   x in s
 }
 
-predicate Trivial5<X(!new)>(older x: X, s: set<X>) {
+ghost predicate Trivial5<X(!new)>(older x: X, s: set<X>) {
   x !in s
 }
 
 // ----------------------------------
 
-predicate Simple0<X>(older x: X, s: set<X>) { // error: x is not older
+ghost predicate Simple0<X>(older x: X, s: set<X>) { // error: x is not older
   true
 }
 
-predicate Simple1<X>(older x: X, s: set<X>) {
+ghost predicate Simple1<X>(older x: X, s: set<X>) {
   x in s
 }
 
-predicate Simple2<X>(older x: X, s: set<X>) { // error: x is not older
+ghost predicate Simple2<X>(older x: X, s: set<X>) { // error: x is not older
   x !in s
 }
 
@@ -54,13 +54,13 @@ module Reachable0 {
 
   datatype Path<T> = Empty | Extend(Path, T)
 
-  predicate Reachable(source: Node, sink: Node, S: set<Node>)
+  ghost predicate Reachable(source: Node, sink: Node, S: set<Node>)
     reads S
   {
     exists via: Path<Node> :: ReachableVia(source, via, sink, S)
   }
 
-  predicate ReachableVia(source: Node, older p: Path<Node>, sink: Node, S: set<Node>)
+  ghost predicate ReachableVia(source: Node, older p: Path<Node>, sink: Node, S: set<Node>)
     reads S
     decreases p
   {
@@ -80,13 +80,13 @@ module Reachable1 {
 
   datatype Path<T, Extra> = Empty | Extend(Path, T, Extra)
 
-  predicate Reachable<Extra>(source: Node, sink: Node, S: set<Node>)
+  ghost predicate Reachable<Extra>(source: Node, sink: Node, S: set<Node>)
     reads S
   {
     exists via: Path<Node, Extra> :: ReachableVia(source, via, sink, S)
   }
 
-  predicate ReachableVia<Extra>(source: Node, older p: Path<Node, Extra>, sink: Node, S: set<Node>) // error: cannot prove p is older
+  ghost predicate ReachableVia<Extra>(source: Node, older p: Path<Node, Extra>, sink: Node, S: set<Node>) // error: cannot prove p is older
     reads S
     decreases p
   {
@@ -106,13 +106,13 @@ module Reachable2 {
   type Extra = int
   datatype Path<T, Extra> = Empty | Extend(Path, T, Extra)
 
-  predicate Reachable(source: Node, sink: Node, S: set<Node>)
+  ghost predicate Reachable(source: Node, sink: Node, S: set<Node>)
     reads S
   {
     exists via: Path<Node, Extra> :: ReachableVia(source, via, sink, S)
   }
 
-  predicate ReachableVia(source: Node, older p: Path<Node, Extra>, sink: Node, S: set<Node>)
+  ghost predicate ReachableVia(source: Node, older p: Path<Node, Extra>, sink: Node, S: set<Node>)
     reads S
     decreases p
   {
@@ -132,13 +132,13 @@ module Reachable3 {
 
   datatype Path<T> = Empty | Extend(Path, T)
 
-  predicate Reachable(source: Node, sink: Node, S: set<Node>)
+  ghost predicate Reachable(source: Node, sink: Node, S: set<Node>)
     reads S
   {
     exists via: Path<Node> :: ReachableVia(source, via, sink, S, 5)
   }
 
-  predicate ReachableVia(source: Node, older p: Path<Node>, sink: Node, S: set<Node>, bound: nat) // error: cannot prove p is older
+  ghost predicate ReachableVia(source: Node, older p: Path<Node>, sink: Node, S: set<Node>, bound: nat) // error: cannot prove p is older
     reads S
     decreases p
   {
@@ -159,13 +159,13 @@ module Reachable4 {
 
   datatype Path<T, Extra> = Empty | Extend(Path, T, Extra)
 
-  predicate Reachable<Extra>(source: Node, sink: Node, S: set<Node>)
+  ghost predicate Reachable<Extra>(source: Node, sink: Node, S: set<Node>)
     reads S
   {
     exists via: Path<Node, Extra> :: ReachableVia(source, via, sink, S)
   }
 
-  predicate ReachableVia<Extra>(source: Node, older p: Path<Node, Extra>, sink: Node, S: set<Node>) // error: cannot prove p is older
+  ghost predicate ReachableVia<Extra>(source: Node, older p: Path<Node, Extra>, sink: Node, S: set<Node>) // error: cannot prove p is older
     reads S
     decreases p
   {
@@ -174,7 +174,7 @@ module Reachable4 {
     case Extend(prefix, n, extra) => n in S && sink in n.children && ReachableVia(source, prefix, n, S)
   }
 
-  predicate ReachableViaEnsures<Extra>(source: Node, older p: Path<Node, Extra>, sink: Node, S: set<Node>)
+  ghost predicate ReachableViaEnsures<Extra>(source: Node, older p: Path<Node, Extra>, sink: Node, S: set<Node>)
     reads S
     ensures !ReachableViaEnsures(source, p, sink, S)
     decreases p
@@ -194,13 +194,13 @@ module Reachable5 {
 
   datatype Path<T> = Empty | Extend(Path, T)
 
-  predicate Reachable(source: Node, sink: Node, S: set<Node>)
+  ghost predicate Reachable(source: Node, sink: Node, S: set<Node>)
     reads S
   {
     exists via: Path<Node> :: ReachableVia(source, via, sink, S, S)
   }
 
-  predicate ReachableVia(source: Node, older p: Path<Node>, sink: Node, S: set<Node>, T: set<Node>)
+  ghost predicate ReachableVia(source: Node, older p: Path<Node>, sink: Node, S: set<Node>, T: set<Node>)
     reads S, T
     decreases p
   {
@@ -216,13 +216,13 @@ module Comprehension {
   class C { }
   datatype List<T> = Nil | Cons(T, List<T>)
 
-  predicate ElementsContainedIn<X>(older xs: List<X>, S: set<X>) {
+  ghost predicate ElementsContainedIn<X>(older xs: List<X>, S: set<X>) {
     match xs
     case Nil => true
     case Cons(x, tail) => x in S && ElementsContainedIn(tail, S)
   }
 
-  function Collection<X>(S: set<X>): iset<List<X>> {
+  ghost function Collection<X>(S: set<X>): iset<List<X>> {
     iset xs: List<X> | ElementsContainedIn(xs, S)
   }
 }
@@ -235,22 +235,22 @@ module MoreTests {
   type Y = set<C>
   type X = List<C>
 
-  predicate P(older x: X, y: Y) {
+  ghost predicate P(older x: X, y: Y) {
     match x
     case Nil => true
     case Cons(head, tail) => head in y && P(tail, y)
   }
 
-  function F(y: Y): int {
+  ghost function F(y: Y): int {
     if forall x: X :: P(x, y) ==> G(x, y) == 3 then
       100
     else
       0
   }
 
-  function G(x: X, y: Y): int
+  ghost function G(x: X, y: Y): int
 
-  function Collection(y: Y): iset<X> {
+  ghost function Collection(y: Y): iset<X> {
     iset x: X | P(x, y)
   }
 }
@@ -260,36 +260,36 @@ module MoreTests {
 module VariationsOnPlurals {
   type X
 
-  predicate One_None(older a: X) { // error: x is not older
+  ghost predicate One_None(older a: X) { // error: x is not older
     true
   }
 
-  predicate One_One(older a: X, b: X) { // error: x is not older
+  ghost predicate One_One(older a: X, b: X) { // error: x is not older
     true
   }
 
-  predicate One_Many(older a: X, b: X, c: X) { // error: x is not older
+  ghost predicate One_Many(older a: X, b: X, c: X) { // error: x is not older
     true
   }
 
-  predicate Many_None(older a: X, older b: X) { // error: x is not older
+  ghost predicate Many_None(older a: X, older b: X) { // error: x is not older
     true
   }
 
-  predicate Many_One(older a: X, older b: X, c: X) { // error: x is not older
+  ghost predicate Many_One(older a: X, older b: X, c: X) { // error: x is not older
     true
   }
 
-  predicate Many_Many(older a: X, older b: X, c: X, d: X) { // error: x is not older
+  ghost predicate Many_Many(older a: X, older b: X, c: X, d: X) { // error: x is not older
     true
   }
 
   class C {
-    predicate One_OneWithThis(older a: X) { // error: x is not older
+    ghost predicate One_OneWithThis(older a: X) { // error: x is not older
       true
     }
 
-    predicate One_ManyWithThis(older a: X, b: X) { // error: x is not older
+    ghost predicate One_ManyWithThis(older a: X, b: X) { // error: x is not older
       true
     }
   }
