Test/triggers/auto-triggers-fix-an-issue-listed-in-the-ironclad-notebook.dfy
@@ -15,7 +15,7 @@ type Key = seq<int>
 type Value = seq<int>
 
 type Hashtable = map<Key, Value>
-function HashtableLookup(h: Hashtable, k: Key): Value
+ghost function HashtableLookup(h: Hashtable, k: Key): Value
 
 lemma HashtableAgreement(h1:Hashtable, h2:Hashtable, k:Key)
   requires forall k :: HashtableLookup(h1,k) == HashtableLookup(h2,k) {
